src/IsoCan.v
@@ -211,6 +211,29 @@ Section IsoCan.
       Proof. by case: ht=> //? /eqP ->; rewrite /eqb_b_hterm/= eqxx. Qed.
 
     End Hgraph.
+  Lemma nth_mapzip (T1 T2 : Type) (S0 T0 : eqType) (x0 : S0) (y0 : T0) [s : seq S0] [t : seq T0] (i : nat) :
+    size s = size t -> nth (@Bnode T1 (IsoCan.hash T0 S0) T2 (mkHinput x0 y0)) [seq Bnode (mkHinput an.1 an.2) | an <- zip s t ] i = Bnode (mkHinput (nth x0 s i) (nth y0 t i)).
+  Proof.
+    move=> eqsize.
+    case/orP : (leqVgt (size t) i)=> leq.
+    + suffices notin : (size [seq Bnode (mkHinput an.1 an.2) | an <- zip s t] <= i)%N.
+      by rewrite !nth_default // eqsize.
+      by move=> ? ? ; rewrite size_map size_zip eqsize minn_refl.
+      by rewrite (nth_map (x0,y0)) ?size_zip ?eqsize ?minn_refl // ; congr Bnode; apply/eqP; rewrite eq_i_ch /= nth_zip //= !eqxx.
+  Qed.
+
+  Lemma find_index_eqbb bs s (bn : B) :
+    size s = size bs ->
+    find (eqb_b_hterm bn) [seq Bnode (mkHinput an.1 an.2) | an <- zip bs s] = index bn bs.
+  Proof.
+    elim: bs s => [| a l IHl]; first by move=> ?; rewrite zip0s.
+    by case =>  [//| b l2] /= [eqsize_tl]; rewrite eq_sym IHl //.
+  Qed.
+
+  Lemma hash_nth_mapzip (U V : Type) (S0 T0 : eqType) (x : S0) (y : T0) [s : seq S0] [t : seq T0] (i : nat):
+    size s = size t ->
+    nth (@Bnode U (IsoCan.hash T0 S0) V (mkHinput x y)) [seq Bnode (mkHinput an.1 an.2) | an <- zip s t ] i = Bnode (mkHinput (nth x s i) (nth y t i)).
+  Proof. by apply nth_mapzip. Qed.
 
   End IsoCanAlgorithm.
 End IsoCan.
